Slightly changing the semantics of register files

src/Array.v
@@ -2,43 +2,41 @@ Require Import FMapPositive.
 Require Import NArith. 
 Require Import ZArith. 
 
+Add Rec LoadPath "." as Synthesis. 
 Require Word. 
 
-Module Map := PositiveMap. 
-
 Section t. 
-  Record T (size : nat) X := mk
-    {
-      body : Map.t X;
-      zero : X  
-    }. 
-  
-  Arguments body {size X} _. 
-  Arguments zero {size X} _. 
+  Variable length : nat.
+  Variable X  : Type. 
+  Definition T := Word.T length ->  X. 
 
-  Variable X : Type.
+  Definition set  (v : T) (j: Word.T length) (x: X) : T :=
+    fun i => if Word.eqb i j then x else v i. 
 
-  Definition set {n} (v : T n X) (adr: Word.T n) (x : X) : T n X :=
-    match Z.to_N (Word.val adr)  with 
-        | N0 => mk _ _ (body v) x
-        | Npos p => mk _ _ (Map.add p x (body v)) (zero v)
-        end. 
+  Definition get (v: T) (i : Word.T length) : X :=
+    v i.
 
-  Definition get {n} (v : T n X) (adr: Word.T n) : X :=
-    match Z.to_N (Word.val adr)  with 
-        | N0 => zero v
-        | Npos p => 
-            match Map.find p  (body v) with 
-                | None => zero v
-                | Some x => x
-        end end. 
-  
-  Definition empty n el : T n X := mk _ _ (Map.empty _) el.
+  Lemma gso (v : T)  i j x:
+    Word.eqb i j = false -> 
+    get (set v i x) j = get v j.
+  Proof. 
+    intros; unfold get, set. simpl. 
+    replace (Word.eqb j i) with (Word.eqb i j). rewrite H. auto.
+    rewrite (Bool.eq_iff_eq_true). rewrite ? Word.eqb_correct. intuition.
+  Qed. 
 
-End t. 
+  Lemma gss v i j x: 
+    Word.eqb i j = true -> 
+    get (set v i x) j = x. 
+  Proof. 
+    unfold get, set. intros. 
+    replace (Word.eqb j i) with (Word.eqb i j). rewrite H. auto.
+    rewrite (Bool.eq_iff_eq_true). rewrite ? Word.eqb_correct. intuition.
+  Qed.
+End t.
 
-Arguments get {X n} _ _. 
-Arguments set {X n} _ _ _. 
+Arguments get {length X} _ _. 
+Arguments set {length X} _ _ _ _. 
              
     
 
